Dom.lean
@@ -87,6 +87,7 @@ import Dom.Properties.Counterexample
 import Dom.Observation
 import Dom.Selector.Match
 import Dom.Selector.Api
+import Dom.Selector.Spec
 
 /-!
 # Lean 4 による WHATWG DOM Standard の形式化
